Foundation/Modal/Modality/S5.lean
@@ -9,9 +9,37 @@ section
 
 open Modality Modalities
 
-variable {L : Logic} [L.IsNormal] {M : Modalities} {n : ℕ} {n : ℕ}
+variable {L : Logic} {M : Modalities} {n : ℕ} {n : ℕ}
 
-abbrev ModalReducible (L : Logic) (n : ℕ) (M : Modalities) := ∀ m ∈ Modalities.allOfSize n, ∃ m' ∈ M, m ⤳[L] m'
+/-- In `L`, every `n`-size modality is reduced to some modality in `M` -/
+abbrev ModalReducible (L : Logic) (n : ℕ) (M : Modalities) := ∀ m, m.size = n → ∃ m' ∈ M, m ⤳[L] m'
+
+lemma ModalReducible.of_allOfSize (h : ∀ m, m ∈ allOfSize n → ∃ m' ∈ M, m ⤳[L] m') : ModalReducible L n M := by
+  intro m hm;
+  apply h;
+  exact allOfSize.iff_mem_eq_size.mpr hm;
+
+/-- In `L`, every modality of size less than `n` is reduced to some modality in `M` -/
+abbrev ModalReducibleLe (L : Logic) (n : ℕ) (M : Modalities) := ∀ m, m.size ≤ n → ∃ m' ∈ M, m ⤳[L] m'
+
+lemma ModalReducibleLe.of_allOfSizeLe (h : ∀ m, m ∈ allOfSizeLe n → ∃ m' ∈ M, m ⤳[L] m') : ModalReducibleLe L n M := by
+  intro m hm;
+  apply h;
+  exact allOfSizeLe.iff_mem_le_size.mpr hm;
+
+lemma ModalReducibleLe.of_cumulative (h : ∀ n' ≤ n, ModalReducible L n' M) : ModalReducibleLe L n M := by
+  intro m hm;
+  apply h m.size ?_ m ?_ <;> tauto;
+
+lemma ModalReducibleLe.gt (h : ModalReducibleLe L n M) (hn : n ≥ n'): ModalReducibleLe L n' M := by
+  intro m hm;
+  apply h m (by omega);
+
+
+lemma ModalReducible.of_le (h : ModalReducibleLe L n M) : ModalReducible L n M := by
+  intro m hm;
+  apply h m (by omega);
+
 
 macro "reduce_to " t:term : tactic => `(tactic| focus
   existsi $t;
@@ -21,19 +49,30 @@ macro "reduce_to " t:term : tactic => `(tactic| focus
   . infer_instance;
 )
 
-lemma ModalReducible.reducible_0 (hM : (-) ∈ M) : ModalReducible L 0 M := by
-  simp only [ModalReducible, allOfSize.eq_zero, Finset.mem_singleton, forall_eq];
+section
+
+variable [L.IsNormal]
+
+lemma ModalReducible.reducible_0_of_mem (hM : (-) ∈ M) : ModalReducible L 0 M := by
+  apply of_allOfSize;
+  intro m hm;
+  simp only [allOfSize.eq_zero, Finset.mem_singleton] at hm;
+  subst hm;
   reduce_to (-);
 
-lemma ModalReducible.reducible_1 (hNeg : (∼) ∈ M) (hBox : (□) ∈ M) (hDia : (◇) ∈ M) : ModalReducible L 1 M := by
+lemma ModalReducible.reducible_1_of_mem (hNeg : (∼) ∈ M) (hBox : (□) ∈ M) (hDia : (◇) ∈ M) : ModalReducible L 1 M := by
+  apply of_allOfSize;
+  intro m hm;
   simp only [
-    ModalReducible, allOfSize, Finset.image_singleton, Finset.union_assoc,
-    Finset.mem_union, Finset.mem_singleton, forall_eq_or_imp, forall_eq
-  ];
-  refine ⟨?_, ?_, ?_⟩;
+    allOfSize, Finset.image_singleton, Finset.union_assoc, Finset.mem_union,
+    Finset.mem_singleton
+  ] at hm;
+  rcases hm with (rfl | rfl | rfl);
   . reduce_to (∼);
   . reduce_to (□);
   . reduce_to (◇);
+
+end
 
 end
 
@@ -42,7 +81,7 @@ namespace Logic.S5
 
 set_option linter.style.multiGoal false
 
-variable {m m₁ m₂ : Modality}
+variable {m m₁ m₂ : Modality} {n}
 
 open Entailment
 open Modality
@@ -52,11 +91,11 @@ open Modalities
 
 protected abbrev modalities : Modalities := {-, ∼, □, ◇, ∼□, ∼◇}
 
-lemma modal_reducible_0 : ModalReducible Logic.S5 0 Logic.S5.modalities := ModalReducible.reducible_0 $ by simp;
+lemma modal_reducible_0 : ModalReducible Logic.S5 0 Logic.S5.modalities := ModalReducible.reducible_0_of_mem $ by simp;
 
-lemma modal_reducible_1 : ModalReducible Logic.S5 1 Logic.S5.modalities := ModalReducible.reducible_1 (by simp) (by simp) (by simp)
+lemma modal_reducible_1 : ModalReducible Logic.S5 1 Logic.S5.modalities := ModalReducible.reducible_1_of_mem (by simp) (by simp) (by simp)
 
-instance : (□□) ≅[Logic.S5] (□)  := by
+instance : (□□) ≅[Logic.S5] (□) := by
   apply iff_equivalence_bi_translate.mpr;
   constructor;
   . apply translation_of_axiomInstance (a := 0);
@@ -69,7 +108,7 @@ instance : (□◇) ≅[Logic.S5] (◇) := by
   constructor;
   . apply translation_of_axiomInstance (a := 0); simp;
   . apply translation_of_axiomInstance (a := 0); simp;
-instance : (◇◇) ≅[Logic.S5] (◇)  := by
+instance : (◇◇) ≅[Logic.S5] (◇) := by
   apply iff_equivalence_bi_translate.mpr;
   constructor;
   . apply translation_of_axiomInstance (a := 0);
@@ -85,9 +124,10 @@ instance : (◇□) ≅[Logic.S5] (□) := by
   . apply translation_of_axiomInstance (a := 0); simp;
 
 lemma modal_reducible_2 : ModalReducible Logic.S5 2 S5.modalities := by
+  apply ModalReducible.of_allOfSize;
   intro m hm;
   simp only [
-    Modalities.allOfSize, Finset.image_singleton, Finset.union_assoc, Finset.mem_union,
+    allOfSize, Finset.image_singleton, Finset.union_assoc, Finset.mem_union,
     Finset.mem_image, Finset.mem_singleton, exists_eq_or_imp, exists_eq_left
   ] at hm;
   rcases hm with (rfl | rfl | rfl) | (rfl | rfl | rfl) | (rfl | rfl | rfl);
@@ -102,15 +142,58 @@ lemma modal_reducible_2 : ModalReducible Logic.S5 2 S5.modalities := by
   . reduce_to (◇);
 
 lemma modal_reducible_3 : ModalReducible Logic.S5 3 S5.modalities := by
-  intro m hm₃;
-  rcases Modalities.allOfSize.eq_succ_right hm₃ with ⟨m, hm₂, (rfl | rfl | rfl)⟩;
-  . obtain ⟨m', hm, hm_reducible⟩ := modal_reducible_2 m hm₂;
-    use m';
+  intro m hm;
+  sorry;
+
+lemma modal_reducible_le_3 : ModalReducibleLe Logic.S5 3 S5.modalities := by
+  apply ModalReducibleLe.of_cumulative;
+  intro n hn;
+  match n with
+  | 0 => exact modal_reducible_0;
+  | 1 => exact modal_reducible_1;
+  | 2 => exact modal_reducible_2;
+  | 3 => exact modal_reducible_3;
+
+lemma modal_reducible_le_succ_4 (n) : ModalReducibleLe Logic.S5 (n + 4) S5.modalities := by
+  intro m hm;
+  obtain ⟨m₁, m₂, hm₁, hm₂, rfl⟩ : ∃ m₁ m₂, m₁.size ≤ 3 ∧ m₂.size ≤ n + 1 ∧ m = m₁ + m₂ := by
+    exact split_le (n₁ := 3) (n₂ := n + 1) $ by omega;
+  induction n generalizing m₂ with
+  | zero =>
+    obtain ⟨m₃, hm₃, _⟩ := modal_reducible_le_3 m₁ hm₁;
+    obtain ⟨m₄, hm₄, _⟩ := modal_reducible_le_3 (m₃ + m₂) $ by
+      simp only [add_size];
+      have : m₃.size ≤ 2 := @Modalities.lt_max_size_of_mem _ S5.modalities (by simp) hm₃;
+      omega;
+    use m₄;
     constructor;
     . assumption;
-    . sorry;
-  . sorry;
-  . sorry;
+    . trans (m₃ + m₂);
+      . apply translation_expand_right;
+      . assumption;
+  | succ n ih =>
+    obtain ⟨m₃, m₄, hm₃, hm₄, rfl⟩ := split_right_le₁ hm₂;
+    obtain ⟨m₅, hm₅, _⟩ := @ih m₃ hm₃ (by simp; omega);
+    obtain ⟨m₆, hm₆, _⟩ := modal_reducible_le_3 (m₅ + m₄) $ by
+      simp only [add_size];
+      have : m₅.size ≤ 2 := @Modalities.lt_max_size_of_mem _ S5.modalities (by simp) hm₅;
+      omega;
+    use m₆;
+    constructor;
+    . assumption;
+    . trans (m₅ + m₄);
+      . rw [show (m₁ + (m₃ + m₄)) = ((m₁ + m₃) + m₄) by simp];
+        apply translation_expand_right;
+      . assumption;
+
+lemma modal_reducible_le (n : ℕ) : ModalReducibleLe Logic.S5 n S5.modalities := by
+  match n with
+  | 0 | 1 | 2 | 3 => apply ModalReducibleLe.gt modal_reducible_le_3 (by omega);
+  | n + 4 => apply modal_reducible_le_succ_4;
+
+lemma modal_reducible (n : ℕ) : ModalReducible Logic.S5 n S5.modalities := by
+  apply ModalReducible.of_le;
+  exact modal_reducible_le n;
 
 end Logic.S5
 
